define func_spec type

core/FuncSpec.v
@@ -22,17 +22,42 @@ Notation path := (list ident).
 
 Context `{target : @Target tags_t (@Expression tags_t)}.
 
-Definition hoare_func_modifies (ge : genv) (p : path) (func : @fundef tags_t) (vars : list path) (exts : list path) :=
+Record func_spec_aux : Type := mk_func_spec {
+  func_spec_p : path;
+  func_spec_pre : arg_assertion;
+  func_spec_post : arg_ret_assertion;
+  func_spec_mod_vars : option (list path); (* None means anything can be modified. *)
+  func_spec_mod_exts : list path
+}.
+
+Inductive func_spec : Type :=
+  | fs_base : func_spec_aux -> func_spec
+  | fs_bind {A} : (A -> func_spec) -> func_spec.
+
+Definition func_modifies_vars (ge : genv) (p : path) (func : @fundef tags_t) (vars : list path) :=
   forall st inargs targs st' outargs sig,
     exec_func ge read_ndetbit p st func targs inargs st' outargs sig ->
-    (forall q, ~(In q vars) -> PathMap.get q (get_memory st) = PathMap.get q (get_memory st'))
-    /\ (forall q, ~(In q exts) -> PathMap.get q (snd st) = PathMap.get q (snd st')).
+    forall q, ~(In q vars) -> PathMap.get q (get_memory st) = PathMap.get q (get_memory st').
 
-Definition hoare_func_spec (ge : genv) (p : path) (pre : arg_assertion)
-    (func : @fundef tags_t) (targs : list P4Type) (post : arg_ret_assertion)
-    (vars : list path) (exts : list path) :=
+Definition func_modifies_exts (ge : genv) (p : path) (func : @fundef tags_t) (exts : list path) :=
+  forall st inargs targs st' outargs sig,
+    exec_func ge read_ndetbit p st func targs inargs st' outargs sig ->
+    forall q, ~(In q exts) -> PathMap.get q (snd st) = PathMap.get q (snd st').
+
+Definition fundef_satisfies_spec_aux (ge : genv) (func : fundef) (targs : list (P4Type)) (fs : func_spec_aux) :=
+  let '(mk_func_spec p pre post vars exts) := fs in
   hoare_func ge p pre func targs post
-    /\ hoare_func_modifies ge p func vars exts.
+    /\ (force True (option_map (func_modifies_vars ge p func) vars))
+    /\  func_modifies_exts ge p func exts.
+
+Fixpoint fundef_satisfies_spec (ge : genv) (func : fundef) (targs : list (P4Type)) (fs : func_spec) :=
+  match fs with
+  | fs_base fs =>
+      fundef_satisfies_spec_aux ge func targs fs
+  | @fs_bind A fs =>
+      (* How can we keep binder names? *)
+      forall (x : A), fundef_satisfies_spec ge func targs (fs x)
+  end.
 
 Definition path_eq_dec : forall (p p' : path), {p = p'} + {p <> p'}.
 Proof.
@@ -49,43 +74,50 @@ Definition hoare_func_frame (ge : genv) (p : path) (pre : arg_assertion) (func :
     post st'.
 
 Lemma hoare_func_frame_intro : forall ge p a_arg a_mem a_ext func targs vars exts a_mem' a_ext',
-  hoare_func_modifies ge p func vars exts ->
-  exclude vars a_mem = a_mem' ->
+  force True (option_map (func_modifies_vars ge p func) vars) ->
+  func_modifies_exts ge p func exts ->
+  force (fun _ => []) (option_map exclude vars) a_mem = a_mem' ->
   exclude exts a_ext = a_ext' ->
   hoare_func_frame ge p (ARG a_arg (MEM a_mem (EXT a_ext))) func targs (MEM a_mem' (EXT a_ext')).
 Proof.
-  unfold hoare_func_modifies, hoare_func_frame; intros.
-  specialize (H _ _  _ _ _ _ H3).
-  destruct H.
+  unfold func_modifies_vars, func_modifies_exts, hoare_func_frame; intros.
+  (* specialize (H _ _  _ _ _ _ H3).
+  destruct H. *)
   destruct st; destruct st'.
-  destruct H2 as [_ []].
+  (* destruct H3 as [_ []]. *)
   split.
-  - clear -H H0 H2.
+  - clear -H H1 H3 H4.
+    destruct vars as [vars | ].
+    2 : { subst; constructor. }
+    specialize (H _ _  _ _ _ _ H4).
+    destruct H3 as [_ []].
     generalize dependent a_mem'.
     induction a_mem; intros.
     + subst. constructor.
-    + simpl in H0. destruct a as [p ?]. destruct (in_dec path_eq_dec p vars) as [H_In | H_In].
+    + simpl in H1. destruct a as [p' ?]. destruct (in_dec path_eq_dec p' vars) as [H_In | H_In].
       * subst; simpl. apply IHa_mem; auto.
-        inv H2; auto.
+        inv H0; auto.
       * subst; simpl. constructor. 
         ++simpl in H; simpl.
           rewrite <- H by auto.
-          inv H2; auto.
+          inv H0; auto.
         ++apply IHa_mem; auto.
-          inv H2; auto.
-  - clear -H1 H5 H4.
+          inv H0; auto.
+  - clear -H0 H2 H3 H4.
     generalize dependent a_ext'.
+    specialize (H0 _ _  _ _ _ _ H4).
+    destruct H3 as [_ []].
     induction a_ext; intros.
     + subst. constructor.
-    + simpl in H1. destruct a as [p ?]. destruct (in_dec path_eq_dec p exts) as [H_In | H_In].
+    + simpl in H2. destruct a as [p' ?]. destruct (in_dec path_eq_dec p' exts) as [H_In | H_In].
       * subst; simpl. apply IHa_ext; auto.
-        inv H5; auto.
+        inv H1; auto.
       * subst; simpl. constructor. 
-        ++simpl in H4; simpl.
-          rewrite <- H4 by auto.
-          inv H5; auto.
+        ++simpl in H0; simpl.
+          rewrite <- H0 by auto.
+          inv H1; auto.
         ++apply IHa_ext; auto.
-          inv H5; auto.
+          inv H1; auto.
 Qed.
 
 Inductive func_post_combine : assertion -> arg_ret_assertion -> arg_ret_assertion -> Prop :=
@@ -115,33 +147,38 @@ Proof.
     eexists; eauto.
 Qed.
 
-Lemma func_spec_combine : forall ge p pre pre' func targs post vars exts post' frame,
+Lemma func_spec_combine : forall ge p pre pre' func targs post post' frame,
   arg_implies pre pre' ->
-  hoare_func_spec ge p pre' func targs post' vars exts ->
+  hoare_func ge p pre' func targs post' ->
   hoare_func_frame ge p pre func targs frame ->
   func_post_combine frame post' post ->
   hoare_func ge p pre func targs post.
 Proof.
   unfold hoare_func; intros.
   specialize (H _ _ H3).
-  destruct H0.
   epose proof (H0 _ _ _ _ _ ltac:(eassumption) ltac:(eassumption)).
-  destruct sig; only 1, 3, 4 : solve [inv H6].
+  destruct sig; only 1, 3, 4 : solve [inv H5].
   eapply (func_post_combine_sound _ _ _ _ _ _ H2); eauto.
 Qed.
 
 Lemma func_spec_combine' : forall ge p pre_arg pre_mem pre_ext pre_arg' pre_mem' pre_ext' func targs post vars exts post' f_mem f_ext,
-  hoare_func_spec ge p (ARG pre_arg' (MEM pre_mem' (EXT pre_ext'))) func targs post' vars exts ->
+  fundef_satisfies_spec_aux ge func targs
+    (mk_func_spec p (ARG pre_arg' (MEM pre_mem' (EXT pre_ext'))) post' vars exts) ->
   arg_implies (ARG pre_arg (MEM pre_mem (EXT pre_ext))) (ARG pre_arg' (MEM pre_mem' (EXT pre_ext'))) ->
-  exclude vars pre_mem = f_mem ->
+  force (fun _ => []) (option_map exclude vars) pre_mem = f_mem ->
   exclude exts pre_ext = f_ext ->
   func_post_combine (MEM f_mem (EXT f_ext)) post' post ->
   hoare_func ge p (ARG pre_arg (MEM pre_mem (EXT pre_ext))) func targs post.
 Proof.
   intros.
+  destruct H as [? []]; eauto.
   eapply func_spec_combine; eauto.
-  destruct H.
   eapply hoare_func_frame_intro; eauto.
 Qed.
 
 End FuncSpec.
+
+Declare Scope func_spec.
+Delimit Scope func_spec with func_spec.
+Notation "'WITH' x .. y , P " :=
+  (fs_bind (fun x => .. (fs_bind (fun y => fs_base P%func_spec)) ..)) (at level 65, x binder, y binder, right associativity) : func_spec.
